io/case-studies/webserver/Monitor.fst
@@ -4,14 +4,34 @@ open FStar.ST
 open MIO.Sig
 open Utils
 
+(* This module is essentially parametric over these, but we must fix them here
+in order to allocate the reference at module initialization time. An alternative
+would be to parametrize the functions by it and pass the reference around. *)
+
+let mst = mymst
+let mi = mymst_impl
+
 private
 val monitor_state : ref mymst.typ
-let monitor_state = ST.alloc my_init_cst
+let monitor_state = ST.alloc mi.init
 
-let get_state () : St mymst.typ = !monitor_state
+let get_state () : St mst.typ = !monitor_state
 
-let update_state (c:caller) (op:io_ops) (argz:io_sig.args op) (rez:io_sig.res op argz) : St unit =
-  let s0 = get_state () in
+(* This function is verified to keep the monitor state related to the trace. The
+(single) caller to this function comes from OCaml code, since it must actually
+have access to the syscalls, and hence the precondition to this function is not
+actually enforced. However, it is easy to see that that function (io_call in
+MIO_Sig_Call.ml) is correct in that it will always update the state after a
+syscall. *)
+
+let update_state
+  (c:caller) (op:io_ops) (argz:io_sig.args op) (rez:io_sig.res op argz)
+  (h : Ghost.erased trace)
+: ST unit
+    (requires fun heap0 -> mst.abstracts (Heap.sel heap0 monitor_state) h)
+    (ensures fun _ _ heap1 -> mst.abstracts (Heap.sel heap1 monitor_state) (convert_call_to_event c op argz rez :: h))
+=
+  let s0 = !monitor_state in
   let e = convert_call_to_event c op argz rez in
-  let s1 = my_update_cst s0 e in
+  let s1 = mi.update s0 e h in
   monitor_state := s1
